programs/lean/Project.lean
@@ -4,4 +4,5 @@ import Project.RustArrayTests.Spec
 import Project.RustU64.Spec
 import Project.RustU64Tests.Spec
 import Project.SwapElements.Spec
+import Project.SwapElements.SwapSepLogic
 import Project.TotalVariation.Spec
